src/proof/k8s_io/apimachinery/pkg/api/meta.v
@@ -1,37 +1,346 @@
 From New.proof Require Import prelude empty_ffi.
 From New.proof.kubernetes_types Require Export prelude.
-From New.proof.k8s_io.api.core Require Export v1_init.
+From New.proof.k8s_io.api.core Require Export v1.
+From New.proof.k8s_io.api.apps Require Export v1.
 From New.proof.k8s_io.apimachinery.pkg.api Require Export meta_init.
+From New.proof.k8s_io.apimachinery.pkg Require Import labels.
 
 Section proof.
 Context `{hG: !heapGS Σ} `{!ffi_semantics _ _}.
 Context {sem : go.Semantics}
-  {package_sem : meta.Assumptions}
+  {package_sem : code.k8s_io.apimachinery.pkg.api.meta.meta.Assumptions}
   {meta_v1_sem : code.k8s_io.apimachinery.pkg.apis.meta.v1.v1.Assumptions}
   {core_v1_sem : code.k8s_io.api.core.v1.v1.Assumptions}
   {apps_v1_sem : code.k8s_io.api.apps.v1.v1.Assumptions}.
 Local Set Default Proof Using "All".
 
-(* FIXME: Accessor should return the same pointer *)
 Lemma wp_Accessor i l o:
-  {{{ is_pkg_init meta ∗
-      ⌜ KObjectV.valid_interface i l o ⌝
+  {{{ "Hinit" ∷ is_pkg_init code.k8s_io.apimachinery.pkg.api.meta.pkg_id.meta ∗
+      "%Hi" ∷ ⌜ KObjectV.valid_interface i l o ⌝
   }}}
-    @! meta.Accessor #(interface.ok i)
-  {{{ RET (#(interface.ok (interface.mk (go.PointerType v1.ObjectMeta) #(KObjectV.objectmeta_ptr l o))), #interface.nil);
+    @! code.k8s_io.apimachinery.pkg.api.meta.meta.Accessor #(interface.ok i)
+  {{{ RET (#(interface.ok i), #interface.nil);
     True
   }}}.
 Proof.
-  (* wp_start as "H". iNamed "H". wp_auto. subst.
-  unshelve wp_apply wp_interface_checked_type_assert; try tc_solve.
-  { iPureIntro. intros Object_id. exists o. done. }
-  iIntros (y ok) "%if_ok".
-  assert (ok = true) as ok_is_true.
-  { destruct ok; [done|]. intuition. }
-  subst ok. inversion if_ok.
-  apply (inj to_val) in H0. subst o.
-  wp_auto. iApply "HΦ". done.
-Qed. *)
-Admitted.
+  wp_start as "H". iNamed "H".
+  destruct o; simpl in Hi; destruct Hi as [-> Hcontains]; wp_auto;
+    rewrite Hcontains; wp_auto.
+  all: iApply "HΦ"; done.
+Qed.
+
+(** The borrowed-labels rule after method promotion through a supported
+    Kubernetes object interface. *)
+Lemma wp_GetLabels_deepown_kobject i l o meta dq :
+  {{{ "Hinit" ∷ is_pkg_init code.k8s_io.apimachinery.pkg.apis.meta.v1.pkg_id.v1 ∗
+      "%Hi" ∷ ⌜ KObjectV.valid_interface i l o ⌝ ∗
+      "Hmeta" ∷ ObjectMetaV.deepown_l (KObjectV.objectmeta_ptr l o) meta dq
+  }}}
+    #(methods i.(interface.ty) "GetLabels" i.(interface.v)) #()
+  {{{ labels_l, RET #labels_l;
+      labels_set_rep labels_l meta.(ObjectMetaV.Labels') dq ∗
+      (labels_set_rep labels_l meta.(ObjectMetaV.Labels') dq -∗
+        ObjectMetaV.deepown_l (KObjectV.objectmeta_ptr l o) meta dq)
+  }}}.
+Proof.
+  wp_start as "H". iNamed "H".
+  destruct o; simpl in Hi; destruct Hi as [-> _]; wp_method_call;
+    wp_pures; wp_apply (wp_GetLabels_deepown with "[$Hinit $Hmeta]");
+    iIntros (labels_l) "Hlabels"; iApply "HΦ"; iFrame.
+Qed.
+
+Lemma wp_GetName_deepown_kobject i l o m dq:
+  {{{ "Hinit" ∷ is_pkg_init code.k8s_io.apimachinery.pkg.apis.meta.v1.pkg_id.v1 ∗
+      "%Hi" ∷ ⌜ KObjectV.valid_interface i l o ⌝ ∗
+      "Hmeta" ∷ ObjectMetaV.deepown_l (KObjectV.objectmeta_ptr l o) m dq
+  }}}
+    #(methods i.(interface.ty) "GetName" i.(interface.v)) #()
+  {{{ RET #m.(ObjectMetaV.Name');
+      ObjectMetaV.deepown_l (KObjectV.objectmeta_ptr l o) m dq
+  }}}.
+Proof.
+  wp_start as "H". iNamed "H".
+  destruct o; simpl in Hi; destruct Hi as [-> _]; wp_method_call;
+    wp_pures; wp_apply (wp_GetName_deepown with "[$Hinit $Hmeta]");
+    iIntros "Hmeta"; iApply "HΦ"; iFrame.
+Qed.
+
+Lemma wp_GetGenerateName_deepown_kobject i l o m dq:
+  {{{ "Hinit" ∷ is_pkg_init code.k8s_io.apimachinery.pkg.apis.meta.v1.pkg_id.v1 ∗
+      "%Hi" ∷ ⌜ KObjectV.valid_interface i l o ⌝ ∗
+      "Hmeta" ∷ ObjectMetaV.deepown_l (KObjectV.objectmeta_ptr l o) m dq
+  }}}
+    #(methods i.(interface.ty) "GetGenerateName" i.(interface.v)) #()
+  {{{ RET #m.(ObjectMetaV.GenerateName');
+      ObjectMetaV.deepown_l (KObjectV.objectmeta_ptr l o) m dq
+  }}}.
+Proof.
+  wp_start as "H". iNamed "H".
+  destruct o; simpl in Hi; destruct Hi as [-> _]; wp_method_call;
+    wp_pures; wp_apply (wp_GetGenerateName_deepown with "[$Hinit $Hmeta]");
+    iIntros "Hmeta"; iApply "HΦ"; iFrame.
+Qed.
+
+Lemma wp_GetUID_deepown_kobject i l o m dq:
+  {{{ "Hinit" ∷ is_pkg_init code.k8s_io.apimachinery.pkg.apis.meta.v1.pkg_id.v1 ∗
+      "%Hi" ∷ ⌜ KObjectV.valid_interface i l o ⌝ ∗
+      "Hmeta" ∷ ObjectMetaV.deepown_l (KObjectV.objectmeta_ptr l o) m dq
+  }}}
+    #(methods i.(interface.ty) "GetUID" i.(interface.v)) #()
+  {{{ RET #m.(ObjectMetaV.UID');
+      ObjectMetaV.deepown_l (KObjectV.objectmeta_ptr l o) m dq
+  }}}.
+Proof.
+  wp_start as "H". iNamed "H".
+  destruct o; simpl in Hi; destruct Hi as [-> _]; wp_method_call;
+    wp_pures; wp_apply (wp_GetUID_deepown with "[$Hinit $Hmeta]");
+    iIntros "Hmeta"; iApply "HΦ"; iFrame.
+Qed.
+
+Lemma wp_GetResourceVersion_deepown_kobject i l o m dq:
+  {{{ "Hinit" ∷ is_pkg_init code.k8s_io.apimachinery.pkg.apis.meta.v1.pkg_id.v1 ∗
+      "%Hi" ∷ ⌜ KObjectV.valid_interface i l o ⌝ ∗
+      "Hmeta" ∷ ObjectMetaV.deepown_l (KObjectV.objectmeta_ptr l o) m dq
+  }}}
+    #(methods i.(interface.ty) "GetResourceVersion" i.(interface.v)) #()
+  {{{ RET #m.(ObjectMetaV.ResourceVersion');
+      ObjectMetaV.deepown_l (KObjectV.objectmeta_ptr l o) m dq
+  }}}.
+Proof.
+  wp_start as "H". iNamed "H".
+  destruct o; simpl in Hi; destruct Hi as [-> _]; wp_method_call;
+    wp_pures; wp_apply (wp_GetResourceVersion_deepown with "[$Hinit $Hmeta]");
+    iIntros "Hmeta"; iApply "HΦ"; iFrame.
+Qed.
+
+Lemma wp_SetName_deepown_kobject i l o m name:
+  {{{ "Hinit" ∷ is_pkg_init code.k8s_io.apimachinery.pkg.apis.meta.v1.pkg_id.v1 ∗
+      "%Hi" ∷ ⌜ KObjectV.valid_interface i l o ⌝ ∗
+      "Hmeta" ∷ ObjectMetaV.deepown_l (KObjectV.objectmeta_ptr l o) m 1
+  }}}
+    #(methods i.(interface.ty) "SetName" i.(interface.v)) #name
+  {{{ RET #();
+      ObjectMetaV.deepown_l (KObjectV.objectmeta_ptr l o)
+        (m <| ObjectMetaV.Name' := name |>) 1
+  }}}.
+Proof.
+  wp_start as "H". iNamed "H".
+  destruct o; simpl in Hi; destruct Hi as [-> _]; wp_method_call;
+    wp_pures; wp_apply (wp_SetName_deepown with "[$Hinit $Hmeta]");
+    iIntros "Hmeta"; iApply "HΦ"; iFrame.
+Qed.
+
+Lemma wp_SetCreationTimestamp_deepown_kobject
+    i l o m creation_timestamp pure_creation_timestamp:
+  {{{ "Hinit" ∷ is_pkg_init code.k8s_io.apimachinery.pkg.apis.meta.v1.pkg_id.v1 ∗
+      "%Hi" ∷ ⌜ KObjectV.valid_interface i l o ⌝ ∗
+      "Hmeta" ∷ ObjectMetaV.deepown_l (KObjectV.objectmeta_ptr l o) m 1 ∗
+      "Htime" ∷ TimeV.deepown creation_timestamp pure_creation_timestamp 1
+  }}}
+    #(methods i.(interface.ty) "SetCreationTimestamp" i.(interface.v))
+      #creation_timestamp
+  {{{ RET #();
+      ObjectMetaV.deepown_l (KObjectV.objectmeta_ptr l o)
+        (m <| ObjectMetaV.CreationTimestamp' := pure_creation_timestamp |>) 1
+  }}}.
+Proof.
+  wp_start as "H". iNamed "H".
+  destruct o; simpl in Hi; destruct Hi as [-> _]; wp_method_call;
+    wp_pures;
+    wp_apply (wp_SetCreationTimestamp_deepown with "[$Hinit $Hmeta $Htime]");
+    iIntros "Hmeta"; iApply "HΦ"; iFrame.
+Qed.
+
+Lemma wp_SetUID_deepown_kobject i l o m uid:
+  {{{ "Hinit" ∷ is_pkg_init code.k8s_io.apimachinery.pkg.apis.meta.v1.pkg_id.v1 ∗
+      "%Hi" ∷ ⌜ KObjectV.valid_interface i l o ⌝ ∗
+      "Hmeta" ∷ ObjectMetaV.deepown_l (KObjectV.objectmeta_ptr l o) m 1
+  }}}
+    #(methods i.(interface.ty) "SetUID" i.(interface.v)) #uid
+  {{{ RET #();
+      ObjectMetaV.deepown_l (KObjectV.objectmeta_ptr l o)
+        (m <| ObjectMetaV.UID' := uid |>) 1
+  }}}.
+Proof.
+  wp_start as "H". iNamed "H".
+  destruct o; simpl in Hi; destruct Hi as [-> _]; wp_method_call;
+    wp_pures; wp_apply (wp_SetUID_deepown with "[$Hinit $Hmeta]");
+    iIntros "Hmeta"; iApply "HΦ"; iFrame.
+Qed.
+
+Lemma wp_SetResourceVersion_deepown_kobject i l o m resource_version:
+  {{{ "Hinit" ∷ is_pkg_init code.k8s_io.apimachinery.pkg.apis.meta.v1.pkg_id.v1 ∗
+      "%Hi" ∷ ⌜ KObjectV.valid_interface i l o ⌝ ∗
+      "Hmeta" ∷ ObjectMetaV.deepown_l (KObjectV.objectmeta_ptr l o) m 1
+  }}}
+    #(methods i.(interface.ty) "SetResourceVersion" i.(interface.v))
+      #resource_version
+  {{{ RET #();
+      ObjectMetaV.deepown_l (KObjectV.objectmeta_ptr l o)
+        (m <| ObjectMetaV.ResourceVersion' := resource_version |>) 1
+  }}}.
+Proof.
+  wp_start as "H". iNamed "H".
+  destruct o; simpl in Hi; destruct Hi as [-> _]; wp_method_call;
+    wp_pures; wp_apply (wp_SetResourceVersion_deepown with "[$Hinit $Hmeta]");
+    iIntros "Hmeta"; iApply "HΦ"; iFrame.
+Qed.
+
+Lemma wp_GetFinalizers_kobject i l o metadata_c dq:
+  {{{ "Hinit" ∷ is_pkg_init code.k8s_io.apimachinery.pkg.apis.meta.v1.pkg_id.v1 ∗
+      "%Hi" ∷ ⌜ KObjectV.valid_interface i l o ⌝ ∗
+      "Hmeta" ∷ (KObjectV.objectmeta_ptr l o) ↦{dq} metadata_c
+  }}}
+    #(methods i.(interface.ty) "GetFinalizers" i.(interface.v)) #()
+  {{{ RET #metadata_c.(code.k8s_io.apimachinery.pkg.apis.meta.v1.v1.ObjectMeta.Finalizers');
+      (KObjectV.objectmeta_ptr l o) ↦{dq} metadata_c
+  }}}.
+Proof.
+  wp_start as "H". iNamed "H".
+  destruct o; simpl in Hi; destruct Hi as [-> _]; wp_method_call;
+    wp_pures; wp_apply (wp_GetFinalizers with "[$Hinit $Hmeta]");
+    iIntros "Hmeta"; iApply "HΦ"; iFrame.
+Qed.
+
+Lemma wp_GetFinalizers_deepown_kobject i l o m dq:
+  {{{ "Hinit" ∷ is_pkg_init code.k8s_io.apimachinery.pkg.apis.meta.v1.pkg_id.v1 ∗
+      "%Hi" ∷ ⌜ KObjectV.valid_interface i l o ⌝ ∗
+      "Hmeta" ∷ ObjectMetaV.deepown_l (KObjectV.objectmeta_ptr l o) m dq
+  }}}
+    #(methods i.(interface.ty) "GetFinalizers" i.(interface.v)) #()
+  {{{ sl, RET #sl;
+      ⌜ sl = slice.nil ↔ m.(ObjectMetaV.Finalizers') = None ⌝ ∗
+      match m.(ObjectMetaV.Finalizers') with
+      | Some vfs => ∃ cfs, sl ↦*{dq} cfs ∗ ⌜ cfs = vfs ⌝ ∗
+          (sl ↦*{dq} cfs -∗ ObjectMetaV.deepown_l (KObjectV.objectmeta_ptr l o) m dq)
+      | None => ObjectMetaV.deepown_l (KObjectV.objectmeta_ptr l o) m dq
+      end
+  }}}.
+Proof.
+  wp_start as "H". iNamed "H".
+  destruct o; simpl in Hi; destruct Hi as [-> _]; wp_method_call;
+    wp_pures; wp_apply (wp_GetFinalizers_deepown with "[$Hinit $Hmeta]");
+    iIntros (sl) "Hfinalizers"; iApply "HΦ"; iFrame.
+Qed.
+
+Lemma wp_SetFinalizers_kobject i l o metadata_c finalizers:
+  {{{ "Hinit" ∷ is_pkg_init code.k8s_io.apimachinery.pkg.apis.meta.v1.pkg_id.v1 ∗
+      "%Hi" ∷ ⌜ KObjectV.valid_interface i l o ⌝ ∗
+      "Hmeta" ∷ (KObjectV.objectmeta_ptr l o) ↦ metadata_c
+  }}}
+    #(methods i.(interface.ty) "SetFinalizers" i.(interface.v)) #finalizers
+  {{{ RET #();
+      (KObjectV.objectmeta_ptr l o) ↦
+        (metadata_c <|
+          code.k8s_io.apimachinery.pkg.apis.meta.v1.v1.ObjectMeta.Finalizers' := finalizers |>)
+  }}}.
+Proof.
+  wp_start as "H". iNamed "H".
+  destruct o; simpl in Hi; destruct Hi as [-> _]; wp_method_call;
+    wp_pures; wp_apply (wp_SetFinalizers with "[$Hinit $Hmeta]");
+    iIntros "Hmeta"; iApply "HΦ"; iFrame.
+Qed.
+
+Lemma wp_GetDeletionGracePeriodSeconds_kobject i l o metadata_c dq:
+  {{{ "Hinit" ∷ is_pkg_init code.k8s_io.apimachinery.pkg.apis.meta.v1.pkg_id.v1 ∗
+      "%Hi" ∷ ⌜ KObjectV.valid_interface i l o ⌝ ∗
+      "Hmeta" ∷ (KObjectV.objectmeta_ptr l o) ↦{dq} metadata_c
+  }}}
+    #(methods i.(interface.ty) "GetDeletionGracePeriodSeconds" i.(interface.v)) #()
+  {{{ RET #metadata_c.(code.k8s_io.apimachinery.pkg.apis.meta.v1.v1.ObjectMeta.DeletionGracePeriodSeconds');
+      (KObjectV.objectmeta_ptr l o) ↦{dq} metadata_c
+  }}}.
+Proof.
+  wp_start as "H". iNamed "H".
+  destruct o; simpl in Hi; destruct Hi as [-> _]; wp_method_call;
+    wp_pures; wp_apply (wp_GetDeletionGracePeriodSeconds with "[$Hinit $Hmeta]");
+    iIntros "Hmeta"; iApply "HΦ"; iFrame.
+Qed.
+
+Lemma wp_SetDeletionGracePeriodSeconds_kobject i l o metadata_c dgps:
+  {{{ "Hinit" ∷ is_pkg_init code.k8s_io.apimachinery.pkg.apis.meta.v1.pkg_id.v1 ∗
+      "%Hi" ∷ ⌜ KObjectV.valid_interface i l o ⌝ ∗
+      "Hmeta" ∷ (KObjectV.objectmeta_ptr l o) ↦ metadata_c
+  }}}
+    #(methods i.(interface.ty) "SetDeletionGracePeriodSeconds" i.(interface.v)) #dgps
+  {{{ RET #();
+      (KObjectV.objectmeta_ptr l o) ↦
+        (metadata_c <|
+          code.k8s_io.apimachinery.pkg.apis.meta.v1.v1.ObjectMeta.DeletionGracePeriodSeconds' := dgps |>)
+  }}}.
+Proof.
+  wp_start as "H". iNamed "H".
+  destruct o; simpl in Hi; destruct Hi as [-> _]; wp_method_call;
+    wp_pures; wp_apply (wp_SetDeletionGracePeriodSeconds with "[$Hinit $Hmeta]");
+    iIntros "Hmeta"; iApply "HΦ"; iFrame.
+Qed.
+
+Lemma wp_GetDeletionTimestamp_kobject i l o metadata_c dq:
+  {{{ "Hinit" ∷ is_pkg_init code.k8s_io.apimachinery.pkg.apis.meta.v1.pkg_id.v1 ∗
+      "%Hi" ∷ ⌜ KObjectV.valid_interface i l o ⌝ ∗
+      "Hmeta" ∷ (KObjectV.objectmeta_ptr l o) ↦{dq} metadata_c
+  }}}
+    #(methods i.(interface.ty) "GetDeletionTimestamp" i.(interface.v)) #()
+  {{{ RET #metadata_c.(code.k8s_io.apimachinery.pkg.apis.meta.v1.v1.ObjectMeta.DeletionTimestamp');
+      (KObjectV.objectmeta_ptr l o) ↦{dq} metadata_c
+  }}}.
+Proof.
+  wp_start as "H". iNamed "H".
+  destruct o; simpl in Hi; destruct Hi as [-> _]; wp_method_call;
+    wp_pures; wp_apply (wp_GetDeletionTimestamp with "[$Hinit $Hmeta]");
+    iIntros "Hmeta"; iApply "HΦ"; iFrame.
+Qed.
+
+Lemma wp_SetDeletionTimestamp_kobject i l o metadata_c deletion_timestamp:
+  {{{ "Hinit" ∷ is_pkg_init code.k8s_io.apimachinery.pkg.apis.meta.v1.pkg_id.v1 ∗
+      "%Hi" ∷ ⌜ KObjectV.valid_interface i l o ⌝ ∗
+      "Hmeta" ∷ (KObjectV.objectmeta_ptr l o) ↦ metadata_c
+  }}}
+    #(methods i.(interface.ty) "SetDeletionTimestamp" i.(interface.v)) #deletion_timestamp
+  {{{ RET #();
+      (KObjectV.objectmeta_ptr l o) ↦
+        (metadata_c <|
+          code.k8s_io.apimachinery.pkg.apis.meta.v1.v1.ObjectMeta.DeletionTimestamp' := deletion_timestamp |>)
+  }}}.
+Proof.
+  wp_start as "H". iNamed "H".
+  destruct o; simpl in Hi; destruct Hi as [-> _]; wp_method_call;
+    wp_pures; wp_apply (wp_SetDeletionTimestamp with "[$Hinit $Hmeta]");
+    iIntros "Hmeta"; iApply "HΦ"; iFrame.
+Qed.
+
+Lemma wp_GetGeneration_kobject i l o metadata_c dq:
+  {{{ "Hinit" ∷ is_pkg_init code.k8s_io.apimachinery.pkg.apis.meta.v1.pkg_id.v1 ∗
+      "%Hi" ∷ ⌜ KObjectV.valid_interface i l o ⌝ ∗
+      "Hmeta" ∷ (KObjectV.objectmeta_ptr l o) ↦{dq} metadata_c
+  }}}
+    #(methods i.(interface.ty) "GetGeneration" i.(interface.v)) #()
+  {{{ RET #metadata_c.(code.k8s_io.apimachinery.pkg.apis.meta.v1.v1.ObjectMeta.Generation');
+      (KObjectV.objectmeta_ptr l o) ↦{dq} metadata_c
+  }}}.
+Proof.
+  wp_start as "H". iNamed "H".
+  destruct o; simpl in Hi; destruct Hi as [-> _]; wp_method_call;
+    wp_pures; wp_apply (wp_GetGeneration with "[$Hinit $Hmeta]");
+    iIntros "Hmeta"; iApply "HΦ"; iFrame.
+Qed.
+
+Lemma wp_SetGeneration_kobject i l o metadata_c generation:
+  {{{ "Hinit" ∷ is_pkg_init code.k8s_io.apimachinery.pkg.apis.meta.v1.pkg_id.v1 ∗
+      "%Hi" ∷ ⌜ KObjectV.valid_interface i l o ⌝ ∗
+      "Hmeta" ∷ (KObjectV.objectmeta_ptr l o) ↦ metadata_c
+  }}}
+    #(methods i.(interface.ty) "SetGeneration" i.(interface.v)) #generation
+  {{{ RET #();
+      (KObjectV.objectmeta_ptr l o) ↦
+        (metadata_c <|
+          code.k8s_io.apimachinery.pkg.apis.meta.v1.v1.ObjectMeta.Generation' := generation |>)
+  }}}.
+Proof.
+  wp_start as "H". iNamed "H".
+  destruct o; simpl in Hi; destruct Hi as [-> _]; wp_method_call;
+    wp_pures; wp_apply (wp_SetGeneration with "[$Hinit $Hmeta]");
+    iIntros "Hmeta"; iApply "HΦ"; iFrame.
+Qed.
 
 End proof.
