src/proof/k8s_io/apimachinery/pkg/apis/meta/v1.v
@@ -1,6 +1,7 @@
 From New.proof.k8s_io.apimachinery.pkg.apis.meta Require Export v1_init.
 From New.proof Require Import prelude empty_ffi.
 From New.proof.kubernetes_types Require Import prelude.
+From New.proof.k8s_io.apimachinery.pkg Require Import labels.
 
 Section proof.
 Context `{hG: !heapGS Σ} `{!ffi_semantics _ _}.
@@ -77,6 +78,65 @@ Proof.
   iFrame.
   iPureIntro.
   done.
+Qed.
+
+(** Borrow the labels map from an owned ObjectMeta. The wand returns the map
+    ownership to the enclosing metadata object after the caller has inspected
+    it. *)
+Lemma wp_GetLabels_deepown meta_l meta dq :
+  {{{ is_pkg_init v1 ∗
+      ObjectMetaV.deepown_l meta_l meta dq
+  }}}
+    meta_l @! (go.PointerType v1.ObjectMeta) @! "GetLabels" #()
+  {{{ labels_l, RET #labels_l;
+      labels_set_rep labels_l meta.(ObjectMetaV.Labels') dq ∗
+      (labels_set_rep labels_l meta.(ObjectMetaV.Labels') dq -∗
+        ObjectMetaV.deepown_l meta_l meta dq)
+  }}}.
+Proof.
+  wp_start as "Hmeta".
+  iDestruct "Hmeta" as (meta_c) "[Hmeta_l Hmeta]".
+  iDestruct (struct_fields_split (V:=v1.ObjectMeta.t) with "Hmeta_l") as
+    "[Hmeta_fields %Hmeta_nonnull]".
+  iNamedPrefix "Hmeta_fields" "Hfield_".
+  iNamed "Hmeta".
+  wp_auto.
+  iApply "HΦ".
+  destruct meta.(ObjectMetaV.Labels') as [label_map|] eqn:Hlabels.
+  - iDestruct "Hdeepown_labels_some" as (label_map_c)
+      "[Hlabel_map %Hlabel_map]". subst label_map_c.
+    iAssert (labels_set_rep meta_c.(v1.ObjectMeta.Labels')
+      (Some label_map) dq) with "[Hlabel_map]" as "Hlabels_rep".
+    { rewrite /labels_set_rep. iFrame.
+      iPureIntro. exact Hdeepown_labels_none. }
+    iFrame "Hlabels_rep".
+    iIntros "Hlabels_rep_back".
+    iEval (rewrite /labels_set_rep) in "Hlabels_rep_back".
+    iDestruct "Hlabels_rep_back" as "[_ Hlabel_map]".
+    iCombineNamed "Hfield_*" as "Hmeta_fields".
+    iAssert (typed_pointsto_def meta_l meta_c dq) with
+      "[Hmeta_fields]" as "Hmeta_l".
+    { iNamed "Hmeta_fields". simpl. rewrite /named. iFrame. }
+    iDestruct (struct_fields_combine (V:=v1.ObjectMeta.t) meta_l meta_c dq
+      Hmeta_nonnull with "Hmeta_l") as "Hmeta_l".
+    iExists meta_c. iFrame "Hmeta_l".
+    rewrite /ObjectMetaV.deepown /named Hlabels. iFrame. iFrame "%".
+    done.
+  - iAssert (labels_set_rep meta_c.(v1.ObjectMeta.Labels') None dq)
+      as "Hlabels_rep".
+    { rewrite /labels_set_rep. iSplit; last done.
+      iPureIntro. split; [intros _; done|].
+      intros _. apply Hdeepown_labels_none. done. }
+    iFrame "Hlabels_rep".
+    iIntros "_".
+    iCombineNamed "Hfield_*" as "Hmeta_fields".
+    iAssert (typed_pointsto_def meta_l meta_c dq) with
+      "[Hmeta_fields]" as "Hmeta_l".
+    { iNamed "Hmeta_fields". simpl. rewrite /named. iFrame. }
+    iDestruct (struct_fields_combine (V:=v1.ObjectMeta.t) meta_l meta_c dq
+      Hmeta_nonnull with "Hmeta_l") as "Hmeta_l".
+    iExists meta_c. iFrame "Hmeta_l".
+    rewrite /ObjectMetaV.deepown /named Hlabels. iFrame. iFrame "%".
 Qed.
 
 Lemma wp_GetGenerateName l m dq :
